Use concrete ivk scalar in address spec

Clean/Orchard/Action.lean
@@ -707,15 +707,15 @@ def Spec (row : Row Ecc.PallasBaseField) : Prop :=
     row.derivedPkDY = row.action.derivedPkDOldY
 
 def OrchardSpec
-    (row : Row Ecc.PallasBaseField)
-    (ivkScalar : ℕ) (gdOld : Ecc.Point Ecc.PallasBaseField) : Prop :=
-  Ecc.IsPallasScalarMulGroupAction ivkScalar gdOld (derivedPkD row) ∧
+    (row : Row Ecc.PallasBaseField) (gdOld : Ecc.Point Ecc.PallasBaseField) : Prop :=
+  Ecc.IsPallasScalarMulGroupAction
+      (Ecc.pallasBaseFieldScalarNat row.ivkScalar) gdOld (derivedPkD row) ∧
     Spec row
 
 theorem spec_of_orchardSpec
     {row : Row Ecc.PallasBaseField}
-    {ivkScalar : ℕ} {gdOld : Ecc.Point Ecc.PallasBaseField}
-    (h : OrchardSpec row ivkScalar gdOld) :
+    {gdOld : Ecc.Point Ecc.PallasBaseField}
+    (h : OrchardSpec row gdOld) :
     Spec row :=
   h.2
 
@@ -741,10 +741,9 @@ theorem pkDOld_scalar_mul_of_derived_scalar_mul
 
 theorem pkDOld_scalar_mul_of_orchardSpec
     {row : Row Ecc.PallasBaseField}
-    {ivkScalar : ℕ}
     {gdOld : Ecc.Point Ecc.PallasBaseField}
-    (hSpec : OrchardSpec row ivkScalar gdOld) :
-    Ecc.IsPallasScalarMul ivkScalar gdOld (pkDOld row) :=
+    (hSpec : OrchardSpec row gdOld) :
+    Ecc.IsPallasBaseFieldScalarMul row.ivkScalar gdOld (pkDOld row) :=
   pkDOld_scalar_mul_of_derived_scalar_mul hSpec.2
     (Ecc.isPallasScalarMul_of_groupAction hSpec.1)
 
@@ -760,10 +759,10 @@ theorem pkDOld_groupAction_of_derived_groupAction
 
 theorem pkDOld_groupAction_of_orchardSpec
     {row : Row Ecc.PallasBaseField}
-    {ivkScalar : ℕ}
     {gdOld : Ecc.Point Ecc.PallasBaseField}
-    (hSpec : OrchardSpec row ivkScalar gdOld) :
-    Ecc.IsPallasScalarMulGroupAction ivkScalar gdOld (pkDOld row) :=
+    (hSpec : OrchardSpec row gdOld) :
+    Ecc.IsPallasScalarMulGroupAction
+      (Ecc.pallasBaseFieldScalarNat row.ivkScalar) gdOld (pkDOld row) :=
   pkDOld_groupAction_of_derived_groupAction hSpec.2 hSpec.1
 
 theorem pkDOld_isPointOrIdentity_of_derived_scalar_mul
